checkout those file that are unrelated to pull

coq/Mini.v
@@ -1,15 +1,11 @@
-Require Export CoqCore.MoreList CoqCore.MoreForall Arith CoqCore.Tactic Omega Program.
+Require Export CoqCore.MoreForall Arith CoqCore.Tactic Omega Program.
 Require Recdef.
 Variable Rest : Type.
 Inductive expr := 
 | If (a b c : expr) 
-| And (l : list expr) 
-| Or (l : list expr)
-| Imply (a b : expr)
-| Not (a : expr)
+| And (a b : expr) 
 | Unknown (R : Rest) (l : list expr)
 | UnknownAtom (R : Rest).
-
 Variable UnknownDenote : Rest -> list expr -> bool.
 Variable UnknownAtomDenote : Rest -> bool.
 Variable RestEqDec : forall l r : Rest, { l = r } + { l <> r }.
@@ -21,22 +17,24 @@ Qed.
 Fixpoint BDenote (e : expr) : bool :=
   match e with
   | If a b c => if BDenote a then BDenote b else BDenote c
-  | And l => forallb BDenote l
-  | Or l => existsb BDenote l
-  | Imply a b => implb (BDenote a) (BDenote b)
-  | Not a => negb (BDenote a)
+  | And a b => BDenote a && BDenote b
   | Unknown R l => UnknownDenote R l
   | UnknownAtom R => UnknownAtomDenote R
+  end.
+
+Fixpoint NumIf (e : expr) :=
+  match e with
+  | If a b c => S (max (max (NumIf a) (NumIf b)) (NumIf c))
+  | And a b => max (NumIf a) (NumIf b)
+  | Unknown R l => fold_left max (map NumIf l) 0
+  | UnknownAtom R => 0
   end.
 
 Fixpoint Size (e : expr) :=
   S 
     match e with
     | If a b c => (Size a + Size b + Size c)
-    | And l => (fold_left plus (map Size l) 0)
-    | Or l => (fold_left plus (map Size l) 0)
-    | Imply a b => (Size a + Size b)
-    | Not a => Size a
+    | And a b => (Size a + Size b)
     | Unknown R l => (fold_left plus (map Size l) 0)
     | UnknownAtom R => 0
     end.
@@ -47,27 +45,24 @@ Qed.
 
 Function IfAndR (ex : expr) { measure Size ex } : expr :=
   match ex with
-  | And [(If a b c); (If d e f)] =>
-      if exprEqDec a d then And [(If a (IfAndR (And [b; e])) (IfAndR (And [c; f])))] else ex
+  | And (If a b c) (If d e f) =>
+      if exprEqDec a d then (If a (IfAndR (And b e)) (IfAndR (And c f))) else ex
+  | And l r => And (IfAndR l) (IfAndR r)
   | _ => ex
   end.
-  all: program_simpl; simpl; omega.
+  all: intros; simpl; subst; omega.
 Qed.
 
 Theorem IfAndRPreserve e : BDenote (IfAndR e) = BDenote e.
   intros.
-  eapply IfAndR_rect; program_simpl.
-  repeat (unfold andb in *; try match_destruct; subst; simpl in *; try congruence).
+  eapply IfAndR_rect; intros; simpl in *; trivial; subst;
+  repeat (try match_destruct; subst; simpl in *; try congruence).
 Qed.
 
 Fixpoint IfAnd (ex : expr) : expr :=
   match ex with
   | If a b c => If (IfAnd a) (IfAnd b) (IfAnd c)
-  | And [l; r] => IfAndR ex
-  | And l => And (map IfAnd l)
-  | Or l => Or (map IfAnd l)
-  | Imply l r => Imply (IfAnd l) (IfAnd r)
-  | Not a => Not (IfAnd a)
+  | And l r => IfAndR ex
   | Unknown r l => Unknown r (map IfAnd l)
   | UnknownAtom r => UnknownAtom r
   end.
@@ -78,31 +73,22 @@ Variable RestBDenoteModular : forall R l l',
 Program Fixpoint expr_ind_Forall
   (P : expr -> Prop)
   (PIf : forall a b c, P a -> P b -> P c -> P (If a b c))
-  (PAnd : forall l, Forall P l -> P (And l))
-  (POr : forall l, Forall P l -> P (Or l))
-  (PImply : forall a b, P a -> P b -> P (Imply a b))
-  (PNot : forall a, P a -> P (Not a))
+  (PAnd : forall a b, P a -> P b -> P (And a b))
   (PUnknown : forall R l, Forall P l -> P (Unknown R l))
   (PUnknownAtom : forall R, P (UnknownAtom R)) e : P e :=
-  let F := (expr_ind_Forall P PIf PAnd POr PImply PNot PUnknown PUnknownAtom) in
+  let F := (expr_ind_Forall P PIf PAnd PUnknown PUnknownAtom) in
     match e with
     | If a b c => PIf a b c (F a) (F b) (F c)
-    | And l => PAnd l (list_ind _ _ (fun ex _ _ => Forall_cons ex (F ex) _) l)
-    | Or l => POr l (list_ind _ _ (fun ex _ _ => Forall_cons ex (F ex) _) l)
-    | Imply a b => PImply a b (F a) (F b)
-    | Not a => PNot a (F a)
+    | And a b => PAnd a b (F a) (F b)
     | Unknown R l => PUnknown R l (list_ind _ _ (fun ex _ _ => Forall_cons ex (F ex) _) l)
     | UnknownAtom R => PUnknownAtom R
     end.
 
-Hint Resolve IfAndRPreserve.
 Definition IfAndPreserve : forall e, BDenote (IfAnd e) = BDenote e.
-  eapply expr_ind_Forall; intros; simpl in *; 
-  try induction l;
-  repeat (
-    unfold implb in *; unfold andb in *;
-    ForallInvcs; try match_destruct; subst; simpl in *; 
-    try rewrite !IfAndRPreserve in *; try congruence).
-  apply RestBDenoteModular; simpl; rewrite H2; f_equal.
-  rewrite map_map; apply map_ext_in; intros; eapply Forall_forall in H3; eauto.
+  eapply expr_ind_Forall; intros; simpl in *; trivial.
+  repeat (try match_destruct; subst; simpl in *; try congruence).
+  apply IfAndRPreserve.
+  apply RestBDenoteModular; rewrite map_map; apply map_ext_in.
+  intros; eapply Forall_forall in H; eauto.
 Qed.
+
